src/phase0/litter.lean
@@ -109,6 +109,9 @@ def near_litter : Type* := Σ i, {s // is_near_litter i s}
 def litter.to_near_litter (i : litter) : near_litter :=
 ⟨i, litter_set i, is_near_litter_litter_set i⟩
 
+lemma litter.to_near_litter_inj : injective litter.to_near_litter :=
+by { intros i j hij, cases hij, refl }
+
 /-- There are `μ` near-litters in total. -/
 @[simp] lemma mk_near_litter : #near_litter = #μ :=
 by { simp only [near_litter, mk_sigma, mk_near_litter', sum_const, mk_litter, lift_id],
